Separated Bag Implementation from Correctness.

src/QueryStructure/Refinements/Bags/BagsInterface.v
@@ -8,9 +8,11 @@ Unset Implicit Arguments.
    *)
 Definition BagInsertEnumerate
            {TContainer TItem: Type}
+           (RepInv : TContainer -> Prop)
            (benumerate : TContainer -> list TItem)
            (binsert    : TContainer -> TItem -> TContainer) :=
   forall inserted container,
+    RepInv container ->
     Permutation
       (benumerate (binsert container inserted))
       (inserted :: benumerate container).
@@ -27,10 +29,12 @@ Definition BagEnumerateEmpty
    using the specified search term [search_term]. *)
 Definition BagFindCorrect
            {TContainer TItem TSearchTerm: Type}
+           (RepInv : TContainer -> Prop)
            (bfind         : TContainer -> TSearchTerm -> list TItem)
            (bfind_matcher : TSearchTerm -> TItem -> bool)
            (benumerate : TContainer -> list TItem) :=
   forall container search_term,
+    RepInv container ->
     Permutation
       (List.filter (bfind_matcher search_term) (benumerate container))
       (bfind container search_term).
@@ -38,6 +42,7 @@ Definition BagFindCorrect
 (* The [bstar] search term matches every item in a bag. *)
 Definition BagFindStar
            {TContainer TItem TSearchTerm: Type}
+           (RepInv : TContainer -> Prop)
            (bfind : TContainer -> TSearchTerm -> list TItem)
            (benumerate : TContainer -> list TItem)
            (bstar : TSearchTerm) :=
@@ -54,9 +59,11 @@ Definition BagUpdateID
    a search term [search_term]. *)
 Definition BagCountCorrect
            {TContainer TItem TSearchTerm: Type}
+           (RepInv : TContainer -> Prop)
            (bcount        : TContainer -> TSearchTerm -> nat)
            (bfind         : TContainer -> TSearchTerm -> list TItem) :=
   forall container search_term,
+    RepInv container ->
     List.length (bfind container search_term) = (bcount container search_term).
 
 (* The elements of a bag [container] from which all elements matching
@@ -64,11 +71,13 @@ Definition BagCountCorrect
    the enumeration of [container] by the negation of [search_term]. *)
 Definition BagDeleteCorrect
            {TContainer TItem TSearchTerm: Type}
+           (RepInv : TContainer -> Prop)
            (bfind         : TContainer -> TSearchTerm -> list TItem)
            (bfind_matcher : TSearchTerm -> TItem -> bool)
            (benumerate : TContainer -> list TItem)
            (bdelete    : TContainer -> TSearchTerm -> (list TItem) * TContainer) :=
   forall container search_term,
+    RepInv container ->
     Permutation (benumerate (snd (bdelete container search_term)))
                 (snd (List.partition (bfind_matcher search_term)
                                      (benumerate container)))
@@ -82,12 +91,14 @@ Definition BagDeleteCorrect
    and matching terms and mapping [f_update] over the latter. *)
 Definition BagUpdateCorrect
            {TContainer TItem TSearchTerm TUpdateTerm : Type}
+           (RepInv : TContainer -> Prop)
            (bfind         : TContainer -> TSearchTerm -> list TItem)
            (bfind_matcher : TSearchTerm -> TItem -> bool)
            (benumerate : TContainer -> list TItem)
            (bupdate_transform : TUpdateTerm -> TItem -> TItem)
            (bupdate    : TContainer -> TSearchTerm -> TUpdateTerm -> TContainer) :=
   forall container search_term update_term,
+    RepInv container ->
     Permutation (benumerate (bupdate container search_term update_term))
                    ((snd (List.partition (bfind_matcher search_term)
                                          (benumerate container)))
@@ -95,32 +106,65 @@ Definition BagUpdateCorrect
                       (fst (List.partition (bfind_matcher search_term)
                                            (benumerate container)))).
 
-Class Bag (TContainer TItem TSearchTerm TUpdateTerm : Type) :=
+Definition binsert_Preserves_RepInv
+           {TContainer TItem: Type}
+           (RepInv : TContainer -> Prop)
+           (binsert    : TContainer -> TItem -> TContainer)
+    := forall container item,
+                        RepInv container
+                        -> RepInv (binsert container item).
+
+Definition bdelete_Preserves_RepInv
+           {TContainer TItem TSearchTerm: Type}
+           (RepInv : TContainer -> Prop)
+           (bdelete    : TContainer -> TSearchTerm -> (list TItem) * TContainer)
+  := forall container search_term,
+                        RepInv container
+                        -> RepInv (snd (bdelete container search_term)).
+
+Definition bupdate_Preserves_RepInv    
+           {TContainer TSearchTerm TUpdateTerm : Type}
+           (RepInv : TContainer -> Prop)
+           (bupdate    : TContainer -> TSearchTerm -> TUpdateTerm -> TContainer)
+  := forall container search_term update_term,
+       RepInv container
+       -> RepInv (bupdate container search_term update_term).
+       
+Class Bag (TItem : Type) :=
   {
-    bempty            : TContainer;
-    bstar             : TSearchTerm;
-    bid               : TUpdateTerm;
-    bfind_matcher     : TSearchTerm -> TItem -> bool;
-    bupdate_transform : TUpdateTerm -> TItem -> TItem;
+    BagType : Type;
+    SearchTermType : Type;
+    UpdateTermType : Type;
 
-    benumerate : TContainer -> list TItem;
-    bfind      : TContainer -> TSearchTerm -> list TItem;
-    binsert    : TContainer -> TItem -> TContainer;
-    bcount     : TContainer -> TSearchTerm -> nat;
-    bdelete    : TContainer -> TSearchTerm -> (list TItem) * TContainer;
-    bupdate    : TContainer -> TSearchTerm -> TUpdateTerm -> TContainer;
+    bempty            : BagType;
+    bstar             : SearchTermType;
+    bid               : UpdateTermType;
+    bfind_matcher     : SearchTermType -> TItem -> bool;
+    bupdate_transform : UpdateTermType -> TItem -> TItem;
 
-    binsert_enumerate : BagInsertEnumerate benumerate binsert;
-    benumerate_empty  : BagEnumerateEmpty benumerate bempty;
-    bfind_star        : BagFindStar bfind benumerate bstar;
-    bfind_correct     : BagFindCorrect bfind bfind_matcher benumerate;
-    bcount_correct    : BagCountCorrect bcount bfind;
-    bdelete_correct   : BagDeleteCorrect bfind bfind_matcher benumerate bdelete;
-    bupdate_correct   : BagUpdateCorrect bfind bfind_matcher benumerate bupdate_transform bupdate
+    benumerate : BagType -> list TItem;
+    bfind      : BagType -> SearchTermType -> list TItem;
+    binsert    : BagType -> TItem -> BagType;
+    bcount     : BagType -> SearchTermType -> nat;
+    bdelete    : BagType -> SearchTermType -> (list TItem) * BagType;
+    bupdate    : BagType -> SearchTermType -> UpdateTermType -> BagType
   }.
 
-Record BagPlusBagProof {TItem} :=
-  { BagType: Type;
-    SearchTermType: Type;
-    UpdateTermType: Type;
-    BagProof: Bag BagType TItem SearchTermType UpdateTermType}.
+
+Class CorrectBag {TItem} (BagImplementation : Bag TItem) :=
+{
+  RepInv            : BagType -> Prop;
+
+  bempty_RepInv     : RepInv bempty;
+  binsert_RepInv    : binsert_Preserves_RepInv RepInv binsert;
+  bdelete_RepInv    : bdelete_Preserves_RepInv RepInv bdelete ;
+  bupdate_RepInv    : bupdate_Preserves_RepInv RepInv bupdate;
+
+  binsert_enumerate : BagInsertEnumerate RepInv benumerate binsert;
+  benumerate_empty  : BagEnumerateEmpty benumerate bempty;
+  bfind_star        : BagFindStar RepInv bfind benumerate bstar;
+  bfind_correct     : BagFindCorrect RepInv bfind bfind_matcher benumerate;
+  bcount_correct    : BagCountCorrect RepInv bcount bfind;
+  bdelete_correct   : BagDeleteCorrect RepInv bfind bfind_matcher benumerate bdelete;
+  bupdate_correct   : BagUpdateCorrect RepInv bfind bfind_matcher benumerate bupdate_transform bupdate
+}.
